v0.1 5/n: allocate_slab WIP

src/Slabs.fst
@@ -550,6 +550,19 @@ let dataify
   Seq.map_seq f s
 
 #push-options "--z3rlimit 30"
+let ind_varraylist (#a: Type)
+  (pred1 pred2 pred3: a -> prop) (r: A.array (AL.cell a))
+  (r1 r2 r3: ref US.t)
+  //(hd1 hd2 hd3: nat)
+  =
+  (vptr r1 `star` vptr r2 `star` vptr r3) `vdep`
+  (fun (idxs: (US.t & US.t) & US.t) ->
+    AL.varraylist pred1 pred2 pred3 r
+    (US.v (fst (fst idxs)))
+    (US.v (snd (fst idxs)))
+    (US.v (snd idxs))
+  )
+
 let s_vprop
   (size_class: sc)
   (slab_region: array U8.t{A.length slab_region = U32.v metadata_max * U32.v page_size})
@@ -570,6 +583,26 @@ let s_vprop
       (f_lemma size_class slab_region md_bm_region md_count (dataify x))
       (SeqUtils.init_u32_refined (U32.v md_count)))
 
+let s_vprop'
+  (size_class: sc)
+  (slab_region: array U8.t{A.length slab_region = U32.v metadata_max * U32.v page_size})
+  (md_bm_region: array U64.t{A.length md_bm_region = U32.v metadata_max * 4})
+  (md_count: U32.t{0 < U32.v md_count /\ U32.v md_count < U32.v metadata_max})
+  (md_region: array (AL.cell status){A.length md_region = U32.v metadata_max})
+  (r1 r2 r3: ref US.t)
+  =
+  ind_varraylist pred1 pred2 pred3
+    (A.split_l md_region (u32_to_sz md_count))
+    r1 r2 r3
+  `vdep`
+  (fun x ->
+    starseq
+      #(pos:U32.t{U32.v pos < U32.v md_count})
+      #(t size_class)
+      (f size_class slab_region md_bm_region md_count (dataify (dsnd x)))
+      (f_lemma size_class slab_region md_bm_region md_count (dataify (dsnd x)))
+      (SeqUtils.init_u32_refined (U32.v md_count)))
+
 #push-options "--z3rlimit 75"
 assume val allocate_slab_aux_1_full
   (size_class: sc)
@@ -582,7 +615,7 @@ assume val allocate_slab_aux_1_full
   (idx2 idx3: US.t)
   (r1 r2 r3: ref US.t)
   //: Steel (array U8.t)
-  : SteelT (US.t & US.t)
+  : SteelT unit
   (
     vptr r1 `star`
     vptr r2 `star`
@@ -593,31 +626,25 @@ assume val allocate_slab_aux_1_full
     starseq
       #(pos:U32.t{U32.v pos < U32.v md_count})
       #(t size_class)
-      (f size_class slab_region md_bm_region md_count md_region_lv)
-      (f_lemma size_class slab_region md_bm_region md_count md_region_lv)
-      (Seq.slice (SeqUtils.init_u32_refined (U32.v md_count)) 0 (US.v idx1)) `star`
-    f size_class slab_region md_bm_region md_count md_region_lv (U32.uint_to_t (US.v idx1)) `star`
-    starseq
-      #(pos:U32.t{U32.v pos < U32.v md_count})
-      #(t size_class)
-      (f size_class slab_region md_bm_region md_count md_region_lv)
-      (f_lemma size_class slab_region md_bm_region md_count md_region_lv)
-      (Seq.slice (SeqUtils.init_u32_refined (U32.v md_count)) (US.v idx1 + 1) (U32.v md_count))
-  )
-  (fun idxs ->
-    vptr r1 `star`
-    vptr r2 `star`
-    vptr r3 `star`
-    (AL.varraylist pred1 pred2 pred3
-      (A.split_l md_region (u32_to_sz md_count))
-      (US.v (fst idxs)) (US.v idx2) (US.v (snd idxs))) `star`
-    starseq
-      #(pos:U32.t{U32.v pos < U32.v md_count})
-      #(t size_class)
-      (f size_class slab_region md_bm_region md_count (Seq.upd md_region_lv (US.v idx1) 2ul))
-      (f_lemma size_class slab_region md_bm_region md_count (Seq.upd md_region_lv (US.v idx1) 2ul))
+      (f size_class slab_region md_bm_region md_count (Seq.upd (G.reveal md_region_lv) (US.v idx1) 2ul))
+      (f_lemma size_class slab_region md_bm_region md_count (Seq.upd (G.reveal md_region_lv) (US.v idx1) 2ul))
       (SeqUtils.init_u32_refined (U32.v md_count))
   )
+  (fun idxs ->
+    s_vprop' size_class slab_region md_bm_region md_count md_region r1 r2 r3
+  )
+  //=
+  //let idx1' = AL.remove1
+  //  (A.split_l md_region (u32_to_sz md_count))
+  //  (US.v idx1) (US.v idx2) (US.v idx3) idx1 in
+  //let idx2' = AL.insert3
+  //  (A.split_l md_region (u32_to_sz md_count))
+  //  (US.v idx1') (US.v idx2) (US.v idx3) idx1 in
+  //write_in_place
+
+
+
+let a = 42
 
 //#push-options "--compat_pre_typed_indexed_effects"
 //#push-options "--z3rlimit 30"
@@ -764,7 +791,7 @@ assume val allocate_slab_aux_1_full
 
 
 
-#push-options "--z3rlimit 75"
+#push-options "--z3rlimit 75 --compat_pre_typed_indexed_effects"
 let allocate_slab_aux_1
   (size_class: sc)
   (slab_region: array U8.t{A.length slab_region = U32.v metadata_max * U32.v page_size})
@@ -774,8 +801,7 @@ let allocate_slab_aux_1
   (md_region_lv: G.erased (Seq.lseq status (U32.v md_count)))
   (idx1 idx2 idx3: US.t)
   (r1 r2 r3: ref US.t)
-  //: Steel (array U8.t)
-  : Steel unit
+  : Steel (array U8.t)
   (
     vptr r1 `star`
     vptr r2 `star`
@@ -790,14 +816,10 @@ let allocate_slab_aux_1
       (f_lemma size_class slab_region md_bm_region md_count md_region_lv)
       (SeqUtils.init_u32_refined (U32.v md_count))
   )
-  (fun _ -> emp)
-  //(fun r ->
-  //  //A.varray r `star`
-  //  vptr r1 `star`
-  //  vptr r2 `star`
-  //  vptr r3 `star`
-  //  s_vprop size_class slab_region md_bm_region md_count md_region (US.v idx1) (US.v idx2) (US.v idx3)
-  //)
+  (fun r ->
+    A.varray r `star`
+    s_vprop' size_class slab_region md_bm_region md_count md_region r1 r2 r3
+  )
   (requires fun h0 ->
     sel r1 h0 == idx1 /\
     sel r2 h0 == idx2 /\
@@ -820,14 +842,12 @@ let allocate_slab_aux_1
   SeqUtils.init_u32_refined_index (U32.v md_count) (US.v idx1);
   change_slprop_rel
      (f size_class slab_region md_bm_region md_count md_region_lv (Seq.index (SeqUtils.init_u32_refined (U32.v md_count)) (US.v idx1)))
-     //(p_empty size_class slab_region md_bm_region md_count s (U32.uint_to_t (US.v idx1)));
      (p_empty size_class (md_bm_array md_bm_region (U32.uint_to_t (US.v idx1)), slab_array slab_region (U32.uint_to_t (US.v idx1))))
      (fun x y -> x == y)
      (fun _ -> admit ());
   p_empty_unpack size_class 
      (md_bm_array md_bm_region (U32.uint_to_t (US.v idx1)), slab_array slab_region (U32.uint_to_t (US.v idx1)))
      (md_bm_array md_bm_region (U32.uint_to_t (US.v idx1)), slab_array slab_region (U32.uint_to_t (US.v idx1)));
-  //slassert (f size_class slab_region md_bm_region md_count (U32.uint_to_t (US.v idx1)));
   let r = allocate_slot size_class
     (md_bm_array md_bm_region (U32.uint_to_t (US.v idx1)))
     (slab_array slab_region (U32.uint_to_t (US.v idx1)))
@@ -837,26 +857,39 @@ let allocate_slab_aux_1
     (slab_array slab_region (U32.uint_to_t (US.v idx1)))
   in
   if cond then (
-    change_slprop_rel
+   change_slprop_rel
       (slab_vprop size_class
         (slab_array slab_region (U32.uint_to_t (US.v idx1)))
         (md_bm_array md_bm_region (U32.uint_to_t (US.v idx1))))
       (f size_class slab_region md_bm_region md_count (Seq.upd md_region_lv (US.v idx1) 2ul) (Seq.index (SeqUtils.init_u32_refined (U32.v md_count)) (US.v idx1)))
       (fun x y -> x == y)
       (fun _ -> admit ());
-    // need for a better starseq_upd wrapper
-    //admit ();
-    //starseq_pack_s
-    //  #_
-    //  #(pos:U32.t{U32.v pos < U32.v md_count})
-    //  #(t size_class)
-    //  (f size_class slab_region md_bm_region md_count (Seq.upd md_region_lv (US.v idx1) 2ul))
-    //  (f_lemma size_class slab_region md_bm_region md_count (Seq.upd md_region_lv (US.v idx1) 2ul))
-    //  (SeqUtils.init_u32_refined (U32.v md_count))
-    //  (US.v idx1);
-    sladmit ()
+    admit ();
+    starseq_upd_pack
+      #_
+      #(pos:U32.t{U32.v pos < U32.v md_count})
+      #(t size_class)
+      (f size_class slab_region md_bm_region md_count (G.reveal md_region_lv))
+      (f size_class slab_region md_bm_region md_count (Seq.upd (G.reveal md_region_lv) (US.v idx1) 2ul))
+      (f_lemma size_class slab_region md_bm_region md_count (G.reveal md_region_lv))
+      (f_lemma size_class slab_region md_bm_region md_count (Seq.upd (G.reveal md_region_lv) (US.v idx1) 2ul))
+      (SeqUtils.init_u32_refined (U32.v md_count))
+      (SeqUtils.init_u32_refined (U32.v md_count))
+      (US.v idx1);
+    sladmit ();
+    allocate_slab_aux_1_full
+      size_class
+      slab_region
+      md_bm_region
+      md_region
+      md_count
+      md_region_lv
+      idx1 idx2 idx3
+      r1 r2 r3;
+    return r
   ) else (
-    sladmit ()
+    sladmit ();
+    return r
   )
 
 (*)
